<?xml version="1.0" encoding="UTF-8"?>
<rdf:RDF xmlns:dc="http://purl.org/dc/elements/1.1/" xmlns:dct="http://purl.org/dc/terms/"
         xmlns:foaf="http://xmlns.com/foaf/0.1/"
         xmlns:gml="http://www.opengis.net/gml"
         xmlns:skos="http://www.w3.org/2004/02/skos/core#"
         xmlns:rdf="http://www.w3.org/1999/02/22-rdf-syntax-ns#">
   <skos:ConceptScheme rdf:about="4f540362-c23e-41e3-8675-7261bbacdeb5:conceptscheme:1.3.1">
      <dc:identifier>4f540362-c23e-41e3-8675-7261bbacdeb5</dc:identifier>
      <dc:title>WMO Distribution Scope</dc:title>
      <dc:description>WMO Distribution Scope from Codelists for description of metadata datasets compliant with the WMO Core Metadata Profile version 1.3 (derived from ISO/TC 211 19115:2003 and 19139)</dc:description>
      <dc:URI>WMO Core Metadata Profile</dc:URI>
      <dct:modified>2013-07-11</dct:modified>
      <dc:creator>
         <foaf:Organization>
            <foaf:name>WMO</foaf:name>
         </foaf:Organization>
      </dc:creator>
      <dc:publisher>
         <foaf:Organization>
            <foaf:name>WMO Information System, World Meteorological Organization</foaf:name>
         </foaf:Organization>
      </dc:publisher>
      <dct:issued>2015-08-21T13:03:12</dct:issued>
   </skos:ConceptScheme>
   <skos:Concept rdf:about="4f540362-c23e-41e3-8675-7261bbacdeb5:concept:63">
      <skos:prefLabel xml:lang="en">GlobalExchange</skos:prefLabel>
      <skos:inScheme rdf:resource="4f540362-c23e-41e3-8675-7261bbacdeb5:conceptscheme:1.3.1"/>
      <skos:broader rdf:resource="4f540362-c23e-41e3-8675-7261bbacdeb5:concept:55"/>
      <skos:definition xml:lang="en">Data are published for global exchange via the WIS. Data shall be incorporated into the GISC Cache.</skos:definition>
      <skos:scopeNote xml:lang="en">GlobalExchange: Data are published for global exchange via the WIS. Data shall be incorporated into the GISC Cache.</skos:scopeNote>
   </skos:Concept>
   <skos:Concept rdf:about="4f540362-c23e-41e3-8675-7261bbacdeb5:concept:75">
      <skos:prefLabel xml:lang="en">RegionalExchange</skos:prefLabel>
      <skos:inScheme rdf:resource="4f540362-c23e-41e3-8675-7261bbacdeb5:conceptscheme:1.3.1"/>
      <skos:broader rdf:resource="4f540362-c23e-41e3-8675-7261bbacdeb5:concept:55"/>
      <skos:definition xml:lang="en">Data are published for regional exchange via a GISC.</skos:definition>
      <skos:scopeNote xml:lang="en">RegionalExchange: Data are published for regional exchange via a GISC.</skos:scopeNote>
   </skos:Concept>
   <skos:Concept rdf:about="4f540362-c23e-41e3-8675-7261bbacdeb5:concept:87">
      <skos:prefLabel xml:lang="en">OriginatingCentre</skos:prefLabel>
      <skos:inScheme rdf:resource="4f540362-c23e-41e3-8675-7261bbacdeb5:conceptscheme:1.3.1"/>
      <skos:broader rdf:resource="4f540362-c23e-41e3-8675-7261bbacdeb5:concept:55"/>
      <skos:definition xml:lang="en">Data are published for exchange directly via the originating centre.</skos:definition>
      <skos:scopeNote xml:lang="en">OriginatingCentre: Data are published for exchange directly via the originating centre.</skos:scopeNote>
   </skos:Concept>
</rdf:RDF>
